src/tactic/vampire/main.lean
@@ -11,8 +11,8 @@ local notation `v*` := xtrm.vr
 local notation `f*` := xtrm.fn
 local notation `[]*` := xtrm.nil
 local notation h `::*` ts  := xtrm.cons h ts
-local notation `r*`     := atm.rl 
-local notation t `=*` s := atm.eq t s 
+local notation `r*`     := atm.rl
+local notation t `=*` s := atm.eq t s
 local notation p `∨*` q := frm.bin tt p q
 local notation p `∧*` q := frm.bin ff p q
 local notation `∃*` p   := frm.qua tt p
@@ -75,7 +75,29 @@ do child ← io.proc.spawn { stdout := io.process.stdio.piped, ..args },
   when (exitv ≠ 0) $ io.fail $ "process exited with status " ++ repr exitv,
   return buf.to_string
 
-variables {α : Type} 
+variables {α : Type}
+
+inductive rul
+| H : nat → rul
+| R : nat → nat → rul
+| I : nat → vmaps → rul
+| P : nat → nat → rul
+| V : nat → rul
+| W : nat → rul
+
+namespace rul
+
+def repr : rul → string
+| (rul.H k)    := "H." ++ k.repr
+| (rul.V k)    := "V." ++ k.repr
+| (rul.W k)    := "W." ++ k.repr
+| (rul.R k m)  := "R." ++ k.repr ++ "." ++ m.repr
+| (rul.P k m)  := "P." ++ k.repr ++ "." ++ m.repr
+| (rul.I k μs) := "I." ++ k.repr ++ "." ++ μs.repr
+
+instance has_repr : has_repr rul := ⟨repr⟩
+
+end rul
 
 inductive proof (m : mat) : cla → Type
 | H (k : nat) : proof (m.nth k)
@@ -83,7 +105,7 @@ inductive proof (m : mat) : cla → Type
   proof ((ff, a) :: c) →
   proof ((tt, a) :: c) →
   proof c
-| I (μs : vmaps) (c : cla) : 
+| I (μs : vmaps) (c : cla) :
   proof c → proof (c.vsubs μs)
 | P (l : lit) (t s : trm) (c : cla) :
   proof (l :: c) →
@@ -91,8 +113,59 @@ inductive proof (m : mat) : cla → Type
   proof (l.replace t s :: c)
 | V (t : trm) (c : cla) :
   proof ((ff, t =* t) :: c) → proof c
-| S (c d : cla) : 
-  cla.sub c d → proof c → proof d
+| W (c d : cla) :
+  cla.subsumes c d → proof c → proof d
+
+variables {R : rls α} {F : fns α} {V : vas α}
+variables {b : bool} (f g : frm)
+
+lemma holds_cla_of_proof {m : mat}
+  (h0 : ∀ V : vas α, m.holds R F V) :
+  ∀ {c : cla}, proof m c →
+  (∀ V : vas α, c.holds R F V) :=
+begin
+  intros c π,
+  induction π with
+    k
+    t c π1 π2 h1 h2
+    μs c π h1
+    l t s c π σ h1 h2
+    t d h1 h2
+    c d h1 π h2 ,
+  { unfold mat.nth,
+    cases h1 : list.nth m k;
+    unfold option.get_or_else,
+    { apply holds_tautology },
+    intro V, apply h0,
+    apply list.mem_iff_nth.elim_right,
+    refine ⟨_, h1⟩ },
+  { intro V,
+    rcases h1 V with ⟨la, hla1 | hla1, hla2⟩,
+    { rcases h2 V with ⟨lb, hlb1 | hlb1, hlb2⟩,
+      { subst hla1, subst hlb1, cases hla2 hlb2 },
+      refine ⟨_, hlb1, hlb2⟩ },
+    refine ⟨_, hla1, hla2⟩ },
+  { intro V,
+    rw cla.holds_vsubs,
+    apply h1 },
+  { intro V,
+    rcases (list.exists_mem_cons_iff _ _ _).elim_left
+      (h1 V) with h3 | ⟨w, h3, h4⟩,
+    { rcases (list.exists_mem_cons_iff _ _ _).elim_left
+        (h2 V) with h4 | ⟨w, h4, h5⟩,
+      { refine ⟨_, or.inl rfl, _⟩,
+        rw lit.holds_replace h4,
+        exact h3 },
+      refine ⟨w, or.inr h4, h5⟩ },
+    refine ⟨w, or.inr h3, h4⟩ },
+  { intro V,
+    rcases h2 V with ⟨l, h2 | h2, h3⟩,
+    { rw h2 at h3,
+      exfalso, apply h3 rfl },
+    refine ⟨l, h2, h3⟩ },
+  { intro,
+    apply cla.holds_of_subsumes h1 (h2 _) }
+end
 
 open tactic
 
@@ -113,14 +186,14 @@ def xtrm.to_asm : ∀ {b : bool}, xtrm b → string
 | _ (f* k ts)  := ts.to_asm ++ to_asm k ++ "f"
 
 instance trm.has_to_asm : has_to_asm trm :=
-⟨xtrm.to_asm⟩ 
+⟨xtrm.to_asm⟩
 
-def list.to_asm [has_to_asm α] : list α → string 
+def list.to_asm [has_to_asm α] : list α → string
 | []        := "n"
 | (a :: as) := list.to_asm as ++ to_asm a ++ "c"
 
 instance list.has_to_asm [has_to_asm α] : has_to_asm (list α) :=
-⟨list.to_asm⟩  
+⟨list.to_asm⟩
 
 def atm.to_asm : atm → string
 | (r* k ts) := to_asm ts ++ to_asm k ++ "r"
@@ -138,29 +211,51 @@ unsafe_run_io $ io.cmd'
 { cmd := "main.pl",
   args := [to_asm m] }
 
-meta inductive item : Type
-| nl                       : item
-| nm  (n : nat)            : item
-| trm (t : trm)            : item
-| trms (ts : trms)         : item
-| mp (μ : vmap)            : item
-| mps (μs : vmaps)         : item
-| prf (x : expr) (c : cla) : item
+def ln : Type := rul × cla
+
+def ln.repr : ln → string
+| (r, c) := cla.repr c ++ " [" ++ r.repr ++ "]"
+
+instance ln.has_repr : has_repr ln := ⟨ln.repr⟩
+
+def lns.repr : list ln → string
+| []        := ""
+| [l]       := l.repr
+| (l :: ls) := l.repr ++ "\n" ++ lns.repr ls
+
+inductive item : Type
+| nl                      : item
+| nm  (n : nat)           : item
+| trm (t : trm)           : item
+| trms (ts : list trm)    : item
+| mp (μ : vmap)           : item
+| mps (μs : vmaps)        : item
+| atm (a : atm)           : item
+| lit (l : lit)           : item
+| cla (c : cla)           : item
+| rul (r : rul)           : item
+| ln  (l : ln)            : item
+| lns (ls : list ln)      : item
 
 namespace item
- 
-meta def repr : item → string 
-| item.nl        := "()"
-| (item.nm n)    := n.repr
-| (item.trm t)   := t.repr
-| (item.trms ts) := ts.repr
-| (item.mp m)    := "VMAP"
-| (item.mps m)   := "VMAPS"
-| (item.prf x c) := "⟦" ++ c.repr ++ "⟧"
 
-meta instance has_repr : has_repr item := ⟨repr⟩ 
+meta def repr : item → string
+| item.nl          := "[]"
+| (item.nm n)      := n.repr
+| (item.trm t)     := t.repr
+| (item.trms ts)   := ts.repr
+| (item.mp μ)      := μ.repr
+| (item.mps μs)    := μs.repr
+| (item.atm a)     := a.repr
+| (item.lit l)     := l.repr
+| (item.cla c)     := cla.repr c
+| (item.rul r)     := r.repr
+| (item.ln (r, c)) := cla.repr c ++ " [" ++ r.repr ++ "]"
+| (item.lns ls)    := ls.repr
 
-meta instance has_to_format : has_to_format item := ⟨λ x, repr x⟩ 
+meta instance has_repr : has_repr item := ⟨repr⟩
+
+meta instance has_to_format : has_to_format item := ⟨λ x, repr x⟩
 
 end item
 
@@ -173,169 +268,131 @@ meta def vmaps.to_expr : vmaps → expr
 
 set_option eqn_compiler.max_steps 4096
 
-/-
-meta def build_proof_core (m : mat) (mx : expr) :
-  list item → list char → tactic expr
-| (item.prf x _ :: stk) [] := return x
-| stk (' ' :: chs) :=
-  build_proof_core stk chs
-| stk ('\n' :: chs) :=
-  build_proof_core stk chs
-| (item.nm k :: stk) ('H' :: infs) :=
-  let πx := expr.mk_app `(@proof.H) [mx, k.to_expr] in
-  build_proof_core (item.prf πx (m.nth k) :: stk) infs
-| (item.nl :: item.prf πx c :: stk) ('S' :: infs) :=
-  let πx' := expr.mk_app `(@proof.S) [mx, `([] : vmaps), cla.to_expr c, πx] in
-  build_proof_core (item.prf πx' c :: stk) infs
-| (item.mps μs :: item.prf πx c :: stk) ('S' :: infs) :=
-  let c' := c.vsubs μs in
-  let πx' := expr.mk_app `(@proof.S) [mx, μs.to_expr, cla.to_expr c, πx] in
-  build_proof_core (item.prf πx' c' :: stk) infs
-| ((item.prf σx ((tt, a) :: d)) :: (item.prf πx ((ff, b) :: c)) :: stk) ('R' :: infs) :=
-  let πx := expr.mk_app `(@proof.R) [mx, a.to_expr, cla.to_expr c, cla.to_expr d, πx, σx] in
-  build_proof_core (item.prf πx (c ++ d) :: stk) infs
-| (item.nm k :: item.prf πx c :: stk) ('T' :: chs) :=
-  let πx := expr.mk_app `(@proof.T) [mx, k.to_expr, c.to_expr, πx] in
-  build_proof_core (item.prf πx (c.rot k) :: stk) chs
-| ((item.prf πx (l :: _ :: c)) :: stk) ('C' :: chs) :=
-  let πx := expr.mk_app `(@proof.C) [mx, l.to_expr, cla.to_expr c, πx] in
-  build_proof_core (item.prf πx (l :: c) :: stk) chs
-| ( (item.prf σx ((tt, t =* s) :: d)) :: (item.prf πx (l :: c)) :: stk ) ('P' :: chs) :=
-  let ρx := expr.mk_app `(@proof.P) 
-    [mx, l.to_expr, t.to_expr, s.to_expr, cla.to_expr c, cla.to_expr d, πx, σx] in
-  build_proof_core (item.prf ρx (l.replace t s :: c ++ d) :: stk) chs
-| ((item.prf πx ((b, t =* s) :: c)) :: stk) ('Y' :: chs) :=
-  let πx' := expr.mk_app `(@proof.Y) [mx, b.to_expr, t.to_expr, s.to_expr, cla.to_expr c, πx] in
-  build_proof_core (item.prf πx' ((b, s =* t) :: c) :: stk) chs
-| ((item.prf πx ((ff, t =* _) :: c)) :: stk) ('V' :: chs) :=
-  let πx' := expr.mk_app `(@proof.V) [mx, t.to_expr, cla.to_expr c, πx] in
-  build_proof_core (item.prf πx' c :: stk) chs
-| stk ('b' :: chs) :=
-  build_proof_core (item.nm 0 :: stk) chs
-| (item.nm k :: stk) ('0' :: chs) :=
-  build_proof_core (item.nm (k * 2) :: stk) chs
-| (item.nm k :: stk) ('1' :: chs) :=
-  build_proof_core (item.nm ((k * 2) + 1) :: stk) chs
-| (item.nm k :: stk) ('v' :: chs) :=
-  build_proof_core (item.trm (v* k) :: stk) chs
-| (item.nm k :: item.nl :: stk) ('f' :: chs) :=
-  build_proof_core (item.trm (f* k []*) :: stk) chs
-| (item.nm k :: item.trms ts :: stk) ('f' :: chs) :=
-  build_proof_core (item.trm (f* k ts) :: stk) chs
-| stk ('n' :: chs) :=
-  build_proof_core (item.nl :: stk) chs
-| (item.nm k :: item.trm t :: stk) ('m' :: infs) :=
-  build_proof_core (item.mp (k, t) :: stk) infs
-| (item.trm t :: item.nl :: stk) ('c' :: infs) :=
-  build_proof_core (item.trms (t ::* []*) :: stk) infs
-| (item.trm t :: item.trms ts :: stk) ('c' :: infs) :=
-  build_proof_core (item.trms (t ::* ts) :: stk) infs
-| (item.mp μ :: item.nl :: stk) ('c' :: infs) :=
-  build_proof_core (item.mps [μ] :: stk) infs
-| (item.mp μ :: item.mps μs :: stk) ('c' :: infs) :=
-  build_proof_core (item.mps (μ :: μs) :: stk) infs
-| (X :: Y :: _) chs := 
-  trace "Stack top : " >> trace X >> trace Y >> 
+open tactic
+
+meta def decode : list item → list char → tactic (list ln)
+| is (' ' :: chs)  := decode is chs
+| is ('\n' :: chs) := decode is chs
+| is ('b' :: chs)  := decode (item.nm 0 :: is) chs
+-- Binary numbers
+| (item.nm k :: is) ('0' :: chs) :=
+  decode (item.nm (k * 2) :: is) chs
+| (item.nm k :: is) ('1' :: chs) :=
+  decode (item.nm ((k * 2) + 1) :: is) chs
+-- Terms
+| (item.nm k :: is) ('v' :: chs) :=
+  decode (item.trm (v* k) :: is) chs
+| (item.nm k :: item.nl :: is) ('f' :: chs) :=
+  decode (item.trm (f* k []*) :: is) chs
+| (item.nm k :: item.trms ts :: is) ('f' :: chs) :=
+  decode (item.trm (f* k $ trms.of_list ts) :: is) chs
+-- Atoms
+| (item.nm k :: item.nl :: is) ('r' :: chs) :=
+  decode (item.atm (r* k []) :: is) chs
+| (item.nm k :: item.trms ts :: is) ('r' :: chs) :=
+  decode (item.atm (r* k ts) :: is) chs
+| (item.trm s :: item.trm t :: is) ('e' :: chs) :=
+  decode (item.atm (t =* s) :: is) chs
+-- Literals
+| (item.atm a :: is) ('+' :: chs) :=
+  decode (item.lit (tt, a) :: is) chs
+| (item.atm a :: is) ('-' :: chs) :=
+  decode (item.lit (ff, a) :: is) chs
+-- Maps
+| (item.nm k :: item.trm t :: is) ('m' :: infs) :=
+  decode (item.mp (k, t) :: is) infs
+-- Lists
+| is ('n' :: chs)  := decode (item.nl :: is) chs
+| (item.trm t :: item.nl :: is) ('c' :: chs) :=
+   decode (item.trms [t] :: is) chs
+| (item.trm t :: item.trms ts :: is) ('c' :: chs) :=
+  decode (item.trms (t :: ts) :: is) chs
+| (item.mp μ :: item.nl :: is) ('c' :: chs) :=
+   decode (item.mps [μ] :: is) chs
+| (item.mp μ :: item.mps μs :: is) ('c' :: chs) :=
+   decode (item.mps (μ :: μs) :: is) chs
+| (item.lit l :: item.nl :: is) ('c' :: chs) :=
+   decode (item.cla [l] :: is) chs
+| (item.lit l :: item.cla c :: is) ('c' :: chs) :=
+   decode (item.cla (l :: c) :: is) chs
+| (item.ln l :: item.nl :: is) ('c' :: chs) :=
+   decode (item.lns [l] :: is) chs
+| (item.ln l :: item.lns ls :: is) ('c' :: chs) :=
+   decode (item.lns (l :: ls) :: is) chs
+-- Rules
+| (item.nm k :: is) ('H' :: chs) :=
+  decode (item.rul (rul.H k) :: is) chs
+| (item.nm k :: is) ('W' :: chs) :=
+  decode (item.rul (rul.W k) :: is) chs
+| (item.nm k :: is) ('V' :: chs) :=
+  decode (item.rul (rul.V k) :: is) chs
+| (item.nm m :: item.nm k :: is) ('R' :: chs) :=
+  decode (item.rul (rul.R k m) :: is) chs
+| (item.nm m :: item.nm k :: is) ('P' :: chs) :=
+  decode (item.rul (rul.P k m) :: is) chs
+| (item.nm k :: item.mps μs :: is) ('I' :: chs) :=
+  decode (item.rul (rul.I k μs) :: is) chs
+| (item.nm k :: item.nl :: is) ('I' :: chs) :=
+  decode (item.rul (rul.I k []) :: is) chs
+-- Lines
+| (item.rul r :: item.cla c :: is) ('l' :: chs) :=
+  decode (item.ln (r, c) :: is) chs
+| (item.rul r :: item.nl :: is) ('l' :: chs) :=
+  decode (item.ln (r, []) :: is) chs
+| [item.lns ls] [] := return ls
+| (X :: Y :: _) chs :=
+  trace "Stack top : " >> trace X >> trace Y >>
   trace "Remaining proof" >> trace chs >> failed
-| (X :: _) chs := 
+| (X :: _) chs :=
   trace "Stack top : " >> trace X >>
   trace "Remaining proof" >> trace chs >> failed
 | [] chs := trace "Stack empty, remaining proof : " >> trace chs >> failed
--/
 
-variables {R : rls α} {F : fns α} {V : vas α}
-variables {b : bool} (f g : frm)
+meta def mk_prf_expr_core (m : mat) (mx : expr) : list ln → tactic (expr × cla)
+| [] := failed
+| ((rul.H k, d) :: lns) :=
+  if d = m.nth k
+  then return (expr.mk_app `(@proof.H) [mx, k.to_expr], m.nth k)
+  else failed
+| ((rul.V k, _) :: lns) :=
+  let lns' := lns.drop k in
+  do (πx, (ff, t =* _) :: c) ← mk_prf_expr_core lns',
+     return (expr.mk_app `(@proof.V) [mx, trm.to_expr t, cla.to_expr c, πx], c)
+| ((rul.R i j, _) :: lns) :=
+  let lns_i := lns.drop i in
+  let lns_j := lns.drop j in
+  do (πx, (ff, a) :: c) ← mk_prf_expr_core lns_i,
+     (σx, (tt, _) :: _) ← mk_prf_expr_core lns_j,
+     return (expr.mk_app `(@proof.R) [mx, atm.to_expr a, cla.to_expr c, πx, σx], c)
+| ((rul.P i j, _) :: lns) :=
+  let lns_i := lns.drop i in
+  let lns_j := lns.drop j in
+  do (πx, l :: c) ← mk_prf_expr_core lns_i,
+     (σx, (tt, t =* s) :: _) ← mk_prf_expr_core lns_j,
+     let ρx := expr.mk_app `(@proof.P)
+       [mx, l.to_expr, t.to_expr, s.to_expr, cla.to_expr c, πx, σx] ,
+     return (ρx, (l.replace t s :: c))
+| ((rul.I k μs, _) :: lns) :=
+  let lns' := lns.drop k in
+  do (πx, c) ← mk_prf_expr_core lns',
+     let σx := expr.mk_app `(@proof.I) [mx, μs.to_expr, c.to_expr, πx],
+     trace "Inst rule with premise : ", trace k,
+     trace "result : ", trace (cla.repr (c.vsubs μs)),
+     return (σx, c.vsubs μs)
+| ((rul.W k, d) :: lns) :=
+  let lns' := lns.drop k in
+  do (πx, c) ← mk_prf_expr_core lns',
+     let sx := expr.mk_app `(cla.subsumes) [c.to_expr, d.to_expr],
+     let dx := expr.mk_app `(cla.subsumes_decidable) [c.to_expr, d.to_expr],
+     let hx := expr.mk_app `(@of_as_true) [sx, dx, `(trivial)],
+     let σx := expr.mk_app `(@proof.W) [mx, c.to_expr, d.to_expr, hx, πx],
+     return (σx, d)
 
 def normalize (f : frm) : frm :=
 skolemize $ pnf $ f.neg
 
 def clausify (f : frm) : mat :=
 cnf $ frm.strip_fa $ normalize f
-
-lemma lit.holds_vsubs (μs : vmaps) (l : lit) :
-  (l.vsubs μs).holds R F V ↔
-  l.holds R F (V.vsubs F μs) :=
-begin
-  cases l with b a; cases b;
-  simp only [ lit.holds, lit.vsubs, atm.holds_vsubs ]
-end
-
-lemma cla.holds_vsubs {μs : vmaps} {c : cla} :
-  (c.vsubs μs).holds R F V ↔
-  c.holds R F (V.vsubs F μs) :=
-by { apply @list.exists_mem_map_iff,
-     apply lit.holds_vsubs }
-
-open list
-
-lemma holds_cla_of_proof {m : mat}
-  (h0 : ∀ V : vas α, m.holds R F V) :
-  ∀ {c : cla}, proof m c →
-  (∀ V : vas α, c.holds R F V) :=
-begin
-  intros c π, 
-  induction π with
-    k 
-    t c π1 π2 h1 h2
-    μs c π h1
-    l t s c π σ h1 h2
-    t d h1 h2
-    c d h1 π h2
-    --k d π h1
-    --b t s d h1 h2
-    ,
-    /-
-  { unfold mat.nth,
-    cases h1 : list.nth m k;
-    unfold option.get_or_else,
-    { apply holds_tautology },
-    intro V, apply h0,
-    apply list.mem_iff_nth.elim_right,
-    refine ⟨_, h1⟩ },
-  { intro V,
-    rcases h1 V with ⟨t, h2 | h2 | h2, h3⟩;
-    refine ⟨_, _, h3⟩,
-    { left, exact h2 },
-    { left, exact h2 },
-    right, exact h2 },
-  { intro V,
-    apply exists_mem_append.elim_right,
-    rcases h1 V with ⟨la, hla1 | hla1, hla2⟩,
-    { rcases h2 V with ⟨lb, hlb1 | hlb1, hlb2⟩,
-      { subst hla1, subst hlb1, cases hla2 hlb2 },
-      right, refine ⟨_, hlb1, hlb2⟩ },
-    left, refine ⟨_, hla1, hla2⟩ },
-  { intro V,  
-    rw cla.holds_vsubs,
-    apply h1 },
-  { intro V,
-    rcases (h1 V) with ⟨t, ht1, ht2⟩,
-    refine ⟨t, _, ht2⟩,
-    apply mem_rot _ ht1 },
-  { intro V,
-    rcases (exists_mem_cons_iff _ _ _).elim_left 
-      (h1 V) with h3 | ⟨w, h3, h4⟩,
-    { rcases (exists_mem_cons_iff _ _ _).elim_left 
-        (h2 V) with h4 | ⟨w, h4, h5⟩,
-      { refine ⟨_, or.inl rfl, _⟩, 
-        rw lit.holds_replace h4,
-        exact h3 },
-      refine ⟨w, or.inr (mem_append_right _ h4), h5⟩ },
-    refine ⟨w, or.inr (mem_append_left _ h3), h4⟩ },
-  { intro V, cases b;
-    { rcases h2 V with ⟨l, h2 | h2, h3⟩, 
-      { refine ⟨_, or.inl rfl, _⟩, 
-        rw h2 at h3,
-        try { apply ne.symm h3 },
-        try { apply eq.symm h3 } },
-      refine ⟨l, or.inr h2, h3⟩ } },
-  { intro V,
-    rcases h2 V with ⟨l, h2 | h2, h3⟩, 
-    { rw h2 at h3,
-      exfalso, apply h3 rfl },
-    refine ⟨l, h2, h3⟩ }
-    -/
-end
 
 lemma frxffx_of_proof [inhabited α]
   (rn : nat) (R : rls α) (fn : nat) (F : fns α) (f : frm) :
@@ -364,14 +421,14 @@ end
 instance decidable_vnew_eq_zero (f : frm) :
   decidable ((normalize f).vnew = 0) := by apply_instance
 
-meta def build_proof (chs : list char)
-  (αx ix : expr) (f : frm) (m : mat) : tactic expr :=
-do πx ← build_proof_core m m.to_expr [] chs,
-   let rnx : expr := f.rnew.to_expr,
-   let fnx : expr := f.fnew.to_expr,
-   let Rx : expr := `(Rdf %%αx),
-   let Fx : expr := `(@Fdf %%αx %%ix),
-   let fx : expr := f.to_expr,
+meta def mk_prf_expr
+  (αx ix : expr) (f : frm) (m : mat) (ls : list ln) : tactic expr :=
+do (πx, []) ← mk_prf_expr_core m m.to_expr ls,
+   let rnx  : expr := f.rnew.to_expr,
+   let fnx  : expr := f.fnew.to_expr,
+   let Rx   : expr := `(Rdf %%αx),
+   let Fx   : expr := `(@Fdf %%αx %%ix),
+   let fx   : expr := f.to_expr,
    let eqx  : expr := `(frm.vnew (normalize %%fx) = 0 : Prop),
    let decx : expr := expr.mk_app `(vampire.decidable_vnew_eq_zero) [fx],
    let hx   : expr := expr.mk_app `(@of_as_true) [eqx, decx, `(trivial)],
@@ -385,24 +442,25 @@ do desugar,
    ix ← get_inhabitance αx,
    f  ← reify αx,
    let m := clausify f,
-   s ← get_asm m,
-   -- s ← (inp <|> get_asm m),
-   -- x ← build_proof s.data αx ix f m,
-   -- apply x,
+   s ← get_asm m, -- s ← (inp <|> get_asm m),
+   ls ← decode [] s.data,
+   x ← mk_prf_expr αx ix f m ls,
+   apply x,
    -- if inp = none
    -- then trace s
    -- else skip
-   trace s
- 
-example (A B : Prop) : A ∧ B → B ∧ A :=
-by vampire
+   skip
 
-#exit
+-- example (A B : Prop) : A ∧ B → B ∧ A :=
+-- by vampire
+
 variables [inhabited α]
 variables (a c : α) (p q : α → Prop) (r : α → α → Prop)
 
 example : (∀ x, p x → q x) → (∀ x, p x) → q a :=
-by vampire 
+by vampire
+
+
 
 example : (∃ x, p x ∧ r x x) → (∀ x, r x x → q x) → ∃ x, p x ∧ q x :=
 by vampire
@@ -448,9 +506,9 @@ lemma knights_and_knaves (me : α) (knight knave rich poor : α → α)
 by vampire
 
 end vampire
- 
+
 -- open lean.parser interactive vampire tactic
--- 
+--
 -- meta def tactic.interactive.vampire
 --   (ids : parse (many ident))
 --   (inp : option string := none) : tactic unit :=
